add SpMSpV dafny

dafny/spmspv.dfy
@@ -1,3 +1,4 @@
+<<<<<<< HEAD
 predicate contains(arr: array<nat>, target: nat)
   reads arr
 {
@@ -91,3 +92,105 @@ method SpMSpV(X_val: array<int>, X_crd: array<nat>, X_pos: array<nat>, v_pos: ar
 
 
 
+=======
+function sum(X_val : array<int>, X_crd : array<nat>,
+             v_val : array<int>, v_crd : array<nat>, kX : nat, kV : nat, pX_end : nat, pV_end : nat) : (s : int) 
+  reads X_val, X_crd
+  requires X_val.Length == X_crd.Length
+  requires pX_end <= X_crd.Length
+  requires forall i :: 0 <= i < X_crd.Length ==> X_crd[i] < X_val.Length
+  requires 0 <= kX <= X_crd.Length
+
+  reads v_crd, v_val
+  requires v_val.Length == v_crd.Length
+  requires pV_end <= v_crd.Length
+  requires forall i :: 0 <= i < v_crd.Length ==> v_crd[i] < v_val.Length
+  requires 0 <= kV <= v_crd.Length
+
+  ensures (pV_end <= kV || pX_end <= kX) ==> s == 0
+  ensures 
+    kX < pX_end && kV < pV_end ==>
+    X_crd[kX] == v_crd[kV] ==> 
+    s == sum(X_val, X_crd, v_val, v_crd, kX + 1, kV + 1, pX_end, pV_end) + v_val[v_crd[kV]] * X_val[X_crd[kX]]
+  decreases pX_end + pV_end - (kX + kV)
+  {
+    if pV_end <= kV || pX_end <= kX then 
+      0
+    else if X_crd[kX] == v_crd[kV] then 
+      sum(X_val, X_crd, v_val, v_crd, kX + 1, kV + 1, pX_end, pV_end) + v_val[v_crd[kV]] * X_val[X_crd[kX]]
+    else if X_crd[kX] < v_crd[kV] then 
+      sum(X_val, X_crd, v_val, v_crd, kX + 1, kV, pX_end, pV_end)
+    else sum(X_val, X_crd, v_val, v_crd, kX, kV + 1, pX_end, pV_end)
+  }
+
+function min(x : nat, y : nat) : nat {
+  if x <= y then x else y
+}
+
+method SpMSpV(X_val : array<int>, X_crd : array<nat>, X_pos : array<nat>,
+              v_val : array<int>, v_crd : array<nat>, v_pos : array<nat>) returns (y : array<int>)
+  // X requirments 
+  requires X_pos.Length >= 1
+  requires X_val.Length == X_crd.Length
+  requires forall i, j :: 0 <= i < j < X_pos.Length ==> X_pos[i] <= X_pos[j];
+  requires forall i :: 0 <= i < X_crd.Length ==> X_crd[i] < X_val.Length
+  requires forall i :: 0 <= i < X_pos.Length ==> 0 <= X_pos[i] <= X_val.Length
+
+  // v requirments 
+  requires v_pos.Length == 2
+  requires v_val.Length == v_crd.Length
+  requires forall i, j :: 0 <= i < j < v_pos.Length ==> v_pos[i] < v_pos[j];
+  requires forall i :: 0 <= i < v_crd.Length ==> v_crd[i] < v_val.Length
+  requires forall i :: 0 <= i < 2            ==> 0 <= v_pos[i] <= v_val.Length
+
+  ensures y.Length + 1 == X_pos.Length
+  ensures 
+    forall i :: 0 <= i < y.Length ==>
+      y[i] == sum(X_val, X_crd, v_val, v_crd, X_pos[i], v_pos[0], X_pos[i+1], v_pos[1])
+  {
+    var N : nat := X_pos.Length - 1;
+    y := new int[N];
+
+    var n : nat := 0;
+    var kX , pX_end : nat;
+    var kV , pV_end : nat;
+    var kX0, kV0    : nat;
+    var k : nat;
+
+    while n < N
+      invariant n <= y.Length
+      invariant forall i :: 0 <= i < n ==> y[i] == sum(X_val, X_crd, v_val, v_crd, X_pos[i], v_pos[0], X_pos[i+1], v_pos[1])
+      { 
+        y[n]   := 0;
+        kX     := X_pos[n];
+        pX_end := X_pos[n + 1];
+        kV     := v_pos[0];
+        pV_end := v_pos[1];
+
+        while (kX < pX_end && kV < pV_end) 
+        invariant X_pos[n] <= kX <= pX_end
+        invariant v_pos[0] <= kV <= pV_end
+        invariant forall i :: 0 <= i < n ==> y[i] == sum(X_val, X_crd, v_val, v_crd, X_pos[i], v_pos[0], X_pos[i+1], v_pos[1])
+        invariant y[n] + sum(X_val, X_crd, v_val, v_crd, kX, kV, pX_end, pV_end) == sum(X_val, X_crd, v_val, v_crd, X_pos[n], v_pos[0], pX_end, pV_end)
+        decreases pX_end + pV_end - (kX + kV)
+          {
+            kX0 := X_crd[kX];
+            kV0 := v_crd[kV];
+            k := min(kV0, kX0);
+            if (kX0 == k && kV0 == k) {
+              assert (kX0 == kV0);
+              y[n] := y[n] + X_val[kX0] * v_val[kX0];
+              kX := kX + 1;
+              kV := kV + 1;
+            } else if (kX0 == k) {
+              assert(kX0 < kV0);
+              kX := kX + 1;
+            } else if (kV0 == k) {
+              assert(kV0 < kX0);
+              kV := kV + 1;
+            }
+          }
+        n := n + 1;
+      }
+  }
+>>>>>>> c51f6ee (add SpMSpV dafny)
